backend/RTLLSim.v
@@ -29,7 +29,7 @@ Definition state_mem (st:state): mem :=
 (* memory relation *)
 
 Record mrelT_opsT (t:Type): Type := mkmrelT_opsT {
-  sem :> t -> forall (i:WF.t) (s1 s2:state), Prop;
+  sem :> t -> forall (p1 p2:program) (i:WF.t) (s1 s2:state), Prop;
   sem_value :> t -> forall (v1 v2:val), Prop;
   le: t -> t -> Prop;
   le_public: t -> t -> Prop
@@ -51,7 +51,7 @@ Record mrelT_propsT (t:Type) (ops:mrelT_opsT t): Prop := mkmrelT_propsT {
 
 Definition mrelT_ops_equals: mrelT_opsT unit :=
   mkmrelT_opsT
-    (fun _ _ s1 s2 => state_mem s1 = state_mem s2)
+    (fun _ _ _ _ s1 s2 => state_mem s1 = state_mem s2)
     (fun _ v1 v2 => Val.lessdef v1 v2)
     (fun _ _ => True)
     (fun _ _ => True).
@@ -65,7 +65,7 @@ Next Obligation. inv H. auto. Qed.
 
 Definition mrelT_ops_extends: mrelT_opsT unit :=
   mkmrelT_opsT
-    (fun _ _ s1 s2 => Mem.extends (state_mem s1) (state_mem s2))
+    (fun _ _ _ _ s1 s2 => Mem.extends (state_mem s1) (state_mem s2))
     (fun _ v1 v2 => Val.lessdef v1 v2)
     (fun _ _ => True)
     (fun _ _ => True).
@@ -114,7 +114,7 @@ Inductive _state_lsim_or_csim
                 (@common_fundef_dec function) fn_sig
                 ge_src ge_tgt fundef_src fundef_tgt)
     (Hargs: list_forall2 (mrelT_ops.(sem_value) mrel) args_src args_tgt)
-    (Hmrel: mrelT_ops.(sem) mrel i st_src st_tgt)
+    (Hmrel: mrelT_ops.(sem) mrel fprog_src fprog_tgt i st_src st_tgt)
     (Hreturn:
        forall mrel2 i2 st2_src st2_tgt mem2_src mem2_tgt vres_src vres_tgt
               (Hvres: mrelT_ops.(sem_value) mrel2 vres_src vres_tgt)
@@ -123,7 +123,7 @@ Inductive _state_lsim_or_csim
               (Hsound_src: sound_state_ext fprog_src st2_src)
               (Hsound_tgt: sound_state_ext fprog_tgt st2_tgt)
               (Hmrel2_le: mrelT_ops.(le_public) mrel mrel2)
-              (Hst2_mem: mrelT_ops.(sem) mrel2 i2 st2_src st2_tgt),
+              (Hst2_mem: mrelT_ops.(sem) mrel2 fprog_src fprog_tgt i2 st2_src st2_tgt),
          state_lsim mrel2 i2 st2_src st2_tgt)
 .
 
@@ -141,7 +141,7 @@ Inductive _state_lsim
     val_src mem_src (Hst_src: st_src = Returnstate cs_entry_src val_src mem_src)
     val_tgt mem_tgt (Hst_tgt: st_tgt = Returnstate cs_entry_tgt val_tgt mem_tgt)
     (Hval: mrelT_ops.(sem_value) mrel val_src val_tgt)
-    (Hmem: mrelT_ops.(sem) mrel i st_src st_tgt)
+    (Hmem: mrelT_ops.(sem) mrel fprog_src fprog_tgt i st_src st_tgt)
     (Hmrel_le_public: mrelT_ops.(le_public) mrel_entry mrel)
 
 | _state_lsim_step
@@ -154,7 +154,7 @@ Inductive _state_lsim
            (plus step ge_tgt st_tgt evt st2_tgt \/
             star step ge_tgt st_tgt evt st2_tgt /\ WF.rel i2 i) /\
            mrelT_ops.(le) mrel mrel2 /\
-           mrelT_ops.(sem) mrel2 i2 st2_src st2_tgt /\
+           mrelT_ops.(sem) mrel2 fprog_src fprog_tgt i2 st2_src st2_tgt /\
            _state_lsim_or_csim state_lsim mrel2 i2 st2_src st2_tgt)
 .
 Hint Constructors _state_lsim.
@@ -187,7 +187,7 @@ Inductive function_lsim (func_src func_tgt:function): Prop :=
          i
          (Hmrel_init: True) (* TODO *)
          (Hmrel_entry_le: mrelT_ops.(le) mrel_init mrel_entry)
-         (Hmrel_entry: mrelT_ops.(sem) mrel_entry i st_src st_tgt)
+         (Hmrel_entry: mrelT_ops.(sem) mrel_entry fprog_src fprog_tgt i st_src st_tgt)
          (Hargs: list_forall2 (mrelT_ops.(sem_value) mrel_entry) args_src args_tgt)
          (Hst_src: st_src = (Callstate cs_entry_src (Internal func_src) args_src mem_entry_src))
          (Hst_tgt: st_tgt = (Callstate cs_entry_tgt (Internal func_tgt) args_tgt mem_entry_tgt))
